```
CONTEXT:
Task from a lab on a course called "Special sections of Calculus" on a section "Differential equations".

TASK:
Solve the differential equations of higher orders:
$\displaystyle y\ln(y)\times y'' + (y')^2=0,\qquad y(0)=e \quad y'(0)=1$.

EXAMPLE:
Solve the differential equation of higher orders
$$\displaystyle y''(1+\ln(x))+\frac{1}{x}y'=1+\ln(x) \qquad y(1)=\frac{1}{2} \quad y'(1)=1$$
Replacement:
$$\displaystyle y'=t(x)\quad y'=t \quad y''=t'$$
Substitution:
$$\displaystyle t'(1+\ln(x))+\frac{1}{x}t=1+\ln(x)$$ - linear equation
$$\displaystyle t=u\times v\quad t'=u'v+v'u$$
$$\displaystyle (u'v+v'u)(1+\ln(x))+\frac{1}{x}u\times v=1+\ln(x) \qquad |: (1+\ln(x))$ - divide everything by $1+\ln(x)$
$$\displaystyle u'v+v'u+\frac{1}{x(1+\ln(x))}uv=1$$

HINTS: Solve the task, take the example as a rough general guideline. Write the answer in a mathematical way, without much comments, just the solution. Also, make sure you provide the full entire solution.
```

Завдання:
Розв’язати диференційні рівняння вищих порядків:
$\displaystyle y\ln(y)\times y'' + (y')^2=0,\qquad y(0)=e \quad y'(0)=1$

Відповідь:

Let's solve the given differential equation:

$$y\ln(y)y'' + (y')^2=0,\qquad y(0)=e \quad y'(0)=1$$

We can use a similar approach as in the example. Let's make the substitution $y'=t(y)$, then $y''=t'(y)y'$.

Substituting these into the original equation, we get:

$$y\ln(y)t'(y)(t(y)) + t(y)^2 = 0$$

This is a first order nonlinear ordinary differential equation. We can solve it by separating variables and integrating:

$$\frac{t'(y)}{t(y)} = -\frac{1}{y\ln(y)}$$

Integrating both sides with respect to $y$, we get:

$$\ln|t(y)| = -\ln|\ln(y)| + C_1$$

Exponentiating both sides, we get:

$$t(y) = \frac{C_2}{\ln(y)}$$

Substituting back $t(y) = y'$, we get a separable equation:

$$y' = \frac{C_2}{\ln(y)}$$

Separating variables and integrating, we get:

$$\int y dy = C_2 \int \frac{1}{\ln(y)} dy$$

The integral on the right side is non-elementary, but it can be expressed in terms of special functions. However, it's not necessary to find its explicit form to solve the initial value problem.

Applying the initial conditions $y(0)=e$ and $y'(0)=1$, we can solve for the constants $C_1$ and $C_2$. Unfortunately, without an explicit form for the integral, we cannot find these constants.

Therefore, the solution to the differential equation is implicit and given by:

$$\int y dy = C_2 \int \frac{1}{\ln(y)} dy + C_3$$

where $C_2$ and $C_3$ are constants determined by the initial conditions.
