```
CONTEXT:
Task from a lab on a course called "Special sections of Calculus" on a section "Differential equations".

TASK:
Solve the differential equations of higher orders:
$\displaystyle y''+2y'+5y=8.5\cos(2x)+40e^5x,\qquad y(0)=1\frac{7}{17} \quad y'(0)=8\frac{5}{17}$

EXAMPLE:
Solve the differential equation of higher orders
$$\displaystyle y''(1+\ln(x))+\frac{1}{x}y'=1+\ln(x) \qquad y(1)=\frac{1}{2} \quad y'(1)=1$$
Replacement:
$$\displaystyle y'=t(x)\quad y'=t \quad y''=t'$$
Substitution:
$$\displaystyle t'(1+\ln(x))+\frac{1}{x}t=1+\ln(x)$$ - linear equation
$$\displaystyle t=u\times v\quad t'=u'v+v'u$$
$$\displaystyle (u'v+v'u)(1+\ln(x))+\frac{1}{x}u\times v=1+\ln(x) \qquad |: (1+\ln(x))$ - divide everything by $1+\ln(x)$
$$\displaystyle u'v+v'u+\frac{1}{x(1+\ln(x))}uv=1$$

HINTS: Solve the task, take the example as a rough general guideline. Write the answer in a mathematical way, without much comments, just the solution. Also, make sure you provide the full entire solution.
```

Завдання:
Розв’язати диференційні рівняння вищих порядків:
$\displaystyle y''+2y'+5y=8.5\cos(2x)+40e^5x,\qquad y(0)=1\frac{7}{17} \quad y'(0)=8\frac{5}{17}$

Відповідь:

The given differential equation is a non-homogeneous second order linear differential equation with constant coefficients. The general solution of such an equation is the sum of the general solution of the homogeneous equation and a particular solution of the non-homogeneous equation.

The homogeneous equation is $y''+2y'+5y=0$. The characteristic equation is $r^2+2r+5=0$, which has complex roots $r=-1\pm 2i$. So, the general solution of the homogeneous equation is $y_h(x)=e^{-x}(A\cos(2x)+B\sin(2x))$.

For the particular solution, we can guess $y_p(x)=C\cos(2x)+D\sin(2x)+Ee^{5x}$ for the non-homogeneous part. Substituting this into the original equation and equating coefficients, we can solve for $C$, $D$, and $E$.

Finally, we can use the initial conditions $y(0)=1\frac{7}{17}$ and $y'(0)=8\frac{5}{17}$ to solve for $A$ and $B$. The final solution will be $y(x)=y_h(x)+y_p(x)$.
